\subsection{minimal consistency improving}
\begin{definition}[\textbf{Condition up to layer}]
Let $c$ be a condition and $d$ a subcondition of $c$. 
The layer of $d$ is defined as $\lay(d) := \nl(c) - \nl(d) - 1$.

Let $L$ be the set of subconditions of $c$ with layer $k$. 
The \emph{condition up to layer} $k$ of $c$ is the condition which is obtained by replacing each $d = Q(a: P \inj P',e) \in L$ by $d = Q(a: P \inj P',\true)$ if $Q = \exists$ and by $Q(a: P \inj P',\false)$ if $Q = \forall$  in $c$. 
\end{definition}

\begin{definition}[\textbf{layered consistency}]
	Let $G$ be a graph, $p: C_0 \to G$ a morphism, $c$ a condition over $C_0$ and $d$ the condition up to layer $k$ of $c$ with $k \geq 1$. 
	The morphism $p$ \emph{satisfies $c$ up to layer} $k$ if $p$ satisfies $d$ and there is no condition $d'$ up to layer $j > k$ such that $p$ satisfies $d'$. 
	The notation $p \models_k  c$ is used if $p$ satisfies $c$ up to layer $k$. 
	The notation $G \models_k c$ is used if $c$ is a constraint and $p \models_k c$ for $p: \emptyset \to G$. 
\end{definition}

\begin{definition}[\textbf{minimal consistency improving}]
Given a rule $r$, a constraint $c$ and a graph $G$ with $G \models_k c$.
A transformation $G \xRightarrow{r,m} H$ is called \emph{minimal consistency improving} if $H \models_j c$ and $k < j$. 
The rule $r$ is called \emph{minimal consistency improving} if all of its applications are. 

\end{definition}

\begin{lemma}
Let $G$ be a graph, $p: C_0 \to G$ a morphism and $c = Q(a_1: C_0 \inj C_1, \overline{Q}(a_2: C_1 \inj C_2, \ldots))$ a condition over $C_0$ in ANF with $p \models_k c$.
If the subcondition $d$ of $c$ with $\lay(d) = k$ is universally bound, $p \models_k c$ implies $p \models c$.
\end{lemma}
\begin{proof}
Let $c' = Q(a_1: C_0 \inj C_1, \ldots \forall(a_k: C_{k-1} \inj C_k, \false) \ldots)$ be the condition up to layer $k$ of $c$ and $d$ be the subcondition of $c$ with $\lay(d) = k + 1$. 
Since $p \models c'$, there does not exist a morphism $q: C_k \to G$ with $p = q \circ a_k \circ \ldots \circ a_1$.
Thus, there does not exists a morphism $q: C_k \to G$ with $q \not \models d$ and $p = q \circ a_k \circ \ldots \circ a_1$ and $p \models c$ follows immediately. 
\end{proof}
